\documentclass[class=article,crop=false]{standalone} 
\input{../preamble.tex}

\begin{document}
\begin{intuition}
	The Fourier transform is basically the "Fourier coefficient" of the basis function for the integral.
\end{intuition}

\subsection{Notation}
~\begin{enumerate}[label=\arabic*)]
	\item 
		\begin{align*}
			\hat{ f}(m) = \lim_{ L \to \infty} \hat{ f}(m_n) = \lim_{ L \to \infty} \frac{L}{\pi} c_n &= \lim_{ L \to \infty} \frac{L}{\pi} \left( \frac{1}{2L} \int_{-L}^{L} f(x) e^{ - i n\pi x / L}   \right) \ dx \\
														  &= \frac{1}{2\pi} \int_{-\infty}^{\infty} f(x) e^{   i m x }  \ dx  \\
		\end{align*}
		\begin{intuition}
			This is sort of the projection formula, since $ 2\pi$ is the circumference of the unit circle.
		\end{intuition}
	\item 
		~\begin{defn} 
			Define the \allbold{Fourier transform} of $ f(x)$ to be  $ \hat{ f}(m) = \mathcal{F}[f](m)$ where
		\[
			\hat{ f}(m) = \mathcal{F}[f](m) = \frac{1}{2\pi } \int_{-\infty}^{\infty} f(x) e^{ -  i m x } \ \forall \ m \in \rr  
		.\] 
	where the kernel is $ K(x,m)=e^{-imx}$. 
\end{defn}
	\item 
		~\begin{defn}
		Define the \allbold{inverse Fourier transform} of $ \hat{ f}(m)$: $ f(x) = \mathcal{F}^{-1} [\hat{ f}](x)$,
		\[
			f(x) = \mathcal{F}^{-1} [\hat{ f}](x) = \int_{-\infty}^{\infty} \hat{ f}(m) e^{imx} dm \ \forall \ x \in \rr  
		.\] 
		where the kernel is $ \hat{ K}(m,x) = e^{imx}$.
	        \end{defn}
	\item Given $ \hat{ f}(m)$ then $ f(x) =\mathcal{F} ^{-1}[\hat{ f}]$ and given $ f(x)$ then  $ \hat{ f}(m) = \mathcal{F}[f]$.
		\begin{intuition}
			The Fourier transform represents a function $ f(x)$ in a new "coordinate system" using different eigenfunction basis. 
		\end{intuition}
\end{enumerate}

Fun Facts:
~\begin{enumerate}[label=\arabic*)]
	\item If $ \int_{-\infty}^{\infty} |f(x)| dx = M<\infty $ then
		\[
			|\hat{ f}(m)|\leq \frac{1}{2\pi} \int_{-\infty}^{\infty} |f(x)| \cdot |e^{-imx}| dx = \frac{1}{2\pi} \int_{-\infty}^{\infty} |f(x)|dx = \frac{M}{2\pi}   
		.\]
	\item Note that
		\[
			\hat{ f}(0)= \frac{1}{2\pi} \int_{-\infty}^{\infty} f(x) dx  = \frac{1}{2\pi} \cdot [ \text{ area under the curve }f(x) ]
		.\] 
	\item If $ f(x)$ is real then  $ \hat{ f}(m)= \overline{\hat{ f}(m)}$.
	\item If $ f(x)$ is even then  $ \hat{ f}(m)$ is even, likewise for odd.
	\item The data $ f(x)$ is transformed to a representation  $ \hat{ f}(m)$ in the frequency domain.
\end{enumerate}

\begin{eg}[]
Suppose
\begin{equation*}
	f(x)=
\begin{cases}
	A, & -L<x<L\\
	\frac{A}{2}, & x=L \text{ or } x=-L\\
	0, & \text{ else} 
\end{cases}
\end{equation*}
Find the Fourier transform of $ f(x)$.

 \begin{align*}
	 \hat{ f}(m) &= \frac{1}{2\pi} \int_{-\infty}^{\infty} f(x)e^{-imx} dx  \\
	 &= \frac{1}{2\pi} \int_{-L}^{L} A e^{-imx} dx  \\
	 &= \frac{A}{2\pi i m} (e^{imL} - e^{-imL}) \\
	 &= \frac{A}{\pi m } \left( \frac{e^{imL}-e^{-imL}}{2i } \right) \\
	 &= \frac{A}{\pi m } \sin(mL ) \\
	 &= \frac{AL}{ \pi} \cdot \frac{\sin(mL )}{mL } \\
\end{align*}
Define the "sinc function" as $ \sinc = \frac{\sin z}{z }$, then
\[
	\hat{ f}(m) = \frac{AL}{\pi} \sinc(mL) = \mathcal{F}[f](m)
.\] 
Moreover, by applying inverse transform on both sides,
\[
	f(x) = \int_{-\infty}^{\infty} \frac{AL}{\pi } \sinc (mL) e^{imx} dm = \mathcal{F}^{-1}[\hat{ f}](x)
.\] 
\end{eg}

\begin{notation}
	Haberman textbook uses the negative exponential term for the transform, but they are equivalent by a change of variable. 
\end{notation}
\end{document}
