\documentclass[class=article,crop=false]{standalone} 
\input{../preamble.tex}

\begin{document}

\begin{intuition}
	We transform the double integral to triple integral using divergence theorem so we can combine them under the same domain of $ \allbold{ x} $. Now we want to replace flux with temperature function.
\end{intuition}

\begin{defn}[Laplacian]
For 3D, the \allbold{Laplacian} is defined as 
	\[
\nabla ^2 u = \Delta u = u_{xx}+u_{yy}+u_{zz}
.\] 
\end{defn}


Recall Fourier's Law says heat flows from hot to cold in the direction where the temperature differences are the greatest and $ \nabla u$ represents the direction of greatest temperature increases, so
\[
	\vv{ \phi}=-K_0 \cdot  \nabla u \implies \nabla \cdot \vv{ \phi}( \allbold{x} ) = \nabla \cdot (-K_0 \nabla u) = -K_0 \cdot \Delta u
.\] 

Then
\[
	c( \allbold{x} )\rho ( \allbold{x}) \frac{\partial }{\partial t} u( \allbold{x},t ) -K_0 \Delta u - Q( \allbold{x},t )=0
.\] 
Thus \allbold{the heat equation with internal source of energy} is
\[
	c( \allbold{x} )\rho ( \allbold{x}) \frac{\partial }{\partial t} u( \allbold{x},t ) =K_0 \Delta u + Q( \allbold{x},t )
.\] 
Assuming $ Q=0$ and the thermal coefficients are constant, we get
\begin{thm}[3D heat equation]
 \[
\frac{\partial u}{\partial t} = k \Delta u 
.\] 
where $k=\frac{K_0}{c \rho}= $ "thermal diffusivity", with initial condition $ u( \allbold{x},0 )= f ( \allbold{x} )$ and boundary condition $ u( \allbold{x} ,t)= T( \allbold{x},t )$ for $ \allbold{x} \in \partial R $.
\end{thm}
\subsection{Steady State}

~\begin{thm}[Laplace's Equation]
Consider the heat equation with internal source of energy defined above, then if $ u_t=0$ this gives  \allbold{Poisson's Equation}, $ \Delta u = -\frac{Q}{K_0}$, and if $ Q=0$ this yields  \allbold{Laplace's Equation}:
\[
\Delta u = \frac{\partial^2 u}{\partial { x}^2} + \frac{\partial^2 u}{\partial { y}^2} + \frac{\partial^2 u}{\partial { z}^2} =0
.\] 
\end{thm}

\begin{thm}[Laplace's Equation in Cylindrical Coordinates]
Let $  x= r \cos(\theta ), y=r \sin(\theta ), z=z$ then using the Chain Rule, 
\[
	\Delta u = \frac{1}{r} \frac{\partial }{\partial r} \left( r \frac{\partial u}{\partial r}  \right) + \frac{1}{r^2} \frac{\partial^2 u}{\partial { \theta}^2}  + \frac{\partial^2 u}{\partial { z}^2} 
.\] 
\end{thm}

\begin{thm}[Spherical]
\[
	\Delta u = \frac{1}{\rho^2} \frac{\partial }{\partial \rho} \left( \rho^2 \frac{\partial u}{\partial \rho}  \right)+ \frac{1}{\rho^2 \sin(\phi )} \frac{\partial }{\partial \phi} \left( \sin(\phi )\frac{\partial u}{\partial \phi}  \right) + \frac{1}{\rho^2 \sin^2(\phi )} \frac{\partial^2 u}{\partial { \phi}^2}  
.\] 
\end{thm}

\newpage
\section{Solving the Heat Equation}
~\begin{defn}[the Heat Operator]
\begin{enumerate}[label=\arabic*)]
	\item Define the \allbold{heat operator} as 
		\[
			L(u) = \frac{\partial u}{\partial t} -k \frac{\partial^2 u}{\partial { x}^2} 
		.\] 
		for any $ u(x,t)$ in the appropriate function space (once differentiable in $ t$ and twice differentiable in  $ x$).
		Then $ L(u)$ is a linear operator.
	\item The set of functions that satisfy the boundary conditions $ u(0,t)=0=u(L,t)$ form a vector space. That is, if  $ u_i$ satisfy these boundary condition for $ i=1,2$ and if $ u_3(x,t)=c_1 u_1(x,t)+ c_2 u_2(x,t)$ then $ u_3(0,t)=0=u_3(L,t) $ for any $ c_1,c_2 \in \rr$.
\end{enumerate}
\begin{note}[]
	The set of function that satisfy the initial condition $ u(x,0)=f(x) \neq 0$ does NOT form a vector space.
\end{note}
\end{defn}

\subsection{Separation of Variables}
Consider the following boundary value problem, there are three pieces of the full story:
\begin{equation*}
\begin{cases}
	\text{ PDE:} \qquad  \frac{\partial u}{\partial t} =k\frac{\partial^2 u}{\partial { x}^2} , & 0<x<L,t>0\\
	\text{ BC:} \qquad  u(0,t)=0=u(L,t), & t>0\\
	\text{ IC:} \qquad  u(x,0) = f(x), & 0\leq x \leq L 
\end{cases}
\end{equation*}

\begin{intuition}
	We will take the non-zero part of the boundary conditions into the steady-state ODE, so that the PDE forms a vector space and becomes easier to solve.
\end{intuition}
Typically we would assume $ u(x,t)= \overline{u}(x) + v(x,t)$ but in this case $ \overline{u}(x)=0$, so we apply separation of variables directly to $ u(x,t)$. Assume (separable functions wrt $ t$ and  $ x$): $ u(x,t)=F(x) \cdot G(t) \neq 0$ then
\[
	\frac{\partial u}{\partial t} =k\frac{\partial^2 u}{\partial { x}^2} \implies F(x) \frac{d G}{d t} = k \frac{d^2 F}{d { x }^2} G(t) \implies \frac{1}{k} \cdot \frac{G'(t)}{G(t)} = \frac{F''(x)}{F(x)}
.\] 
For this to satisfy, the ratio must be a constant.
\begin{prf}
We aim to show that the derivative of LHS wrt $ t$ is zero for all $ t$. Note that
\[
	\frac{d }{d t} \left( \frac{1}{k} \cdot  \frac{G'(t)}{G(t)} \right) = \frac{d }{d t} \left( \frac{F''(x)}{F(x)} \right) =0
.\]
and likewise for the RHS
\[
	\frac{d }{d x} \left( \frac{F''(x)}{F(x)} \right) =0 
.\] 
Together 0 derivative everywhere implies a constant function:
\[
	\frac{1}{k} \cdot  \frac{G'(t)}{G(t)}=\frac{F''(x)}{F(x)}=-\lambda
.\] 
where $ \lambda$ is some constant. 
\end{prf}
Now consider the differential equations
\[
	G'(t)=-\lambda k G(t) \text{ and } F''(x) = -\lambda F(x) 
.\] 
\end{document}
