\documentclass[class=article,crop=false]{standalone} 
\input{../preamble.tex}

\begin{document}

\begin{equation*}
\begin{cases}
	G''(y) = \lambda G(y)\\
	G(0)=0, G(H)=0\\
\end{cases}
\end{equation*}
and  $F''(x)=-\lambda F(x)$. We do the same process again to solve $ u_2(x,t)$. Note that since only $ \lambda <0$ works to solve to F-equation, we require $ |\lambda|=\left( \frac{n\pi}{H } \right)^2 \implies \lambda = -\left(\frac{n\pi}{H } \right)^2$. The solution is

\[
	u_2(x,y)=\sum_{ n= 1}^{\infty} c_n \sinh\left(\frac{n\pi x}{H }  \right)
	\sin \left( \frac{ n\pi y}{ H} \right) + d_n \sinh\left(\frac{n\pi [x-L]}{H } \right) \sin \left( \frac{ n\pi y}{ H} \right) 
.\] 
with coefficients
\[
	c_n= \frac{\frac{2}{H} \int_0^H g_2(y) \sin \left( \frac{ n\pi y}{ H} \right) dy }{\sinh\left(\frac{n\pi L}{H } \right) } \text{ and } d_n =  \frac{\frac{2}{H} \int_0^H g_1(y) \sin \left( \frac{ n\pi y}{ H} \right) dy }{\sinh\left(\frac{-n\pi L}{H } \right) }
.\] 
Then the \allbold{formal solution} is 
\begin{align*}
	u(x,y) &= u_1(x,y)+u_2(x,y) \\
	&= \sum_{ n= 1}^{\infty} a_n \sinh\left(\frac{n\pi y}{L }  \right) \sin \left( \frac{ n\pi x}{ L} \right) + b_n \sinh\left(\frac{n\pi [y-H]}{L } \right) \sin \left( \frac{ n\pi x}{ L} \right) \\
	&\quad + \sum_{ n= 1}^{\infty} c_n \sinh\left(\frac{n\pi x}{H }  \right) \sin \left( \frac{ n\pi y}{ H} \right) + d_n \sinh\left(\frac{n\pi [x-L]}{H } \right) \sin \left( \frac{ n\pi y}{ H} \right) \\
\end{align*}
with the coefficients:
\begin{align*}
	a_n= \frac{\frac{2}{L} \int_0^L f_2(x) \sin \left( \frac{ n\pi x}{ L} \right) dx }{\sinh\left(\frac{n\pi H}{L } \right) } &\text{ and } b_n =  \frac{\frac{2}{L} \int_0^L f_1(x) \sin \left( \frac{ n\pi x}{ L} \right) dx }{\sinh\left(\frac{-n\pi H}{L } \right) }\\
	c_n= \frac{\frac{2}{H} \int_0^H g_2(y) \sin \left( \frac{ n\pi y}{ H} \right) dy }{\sinh\left(\frac{n\pi L}{H } \right) } &\text{ and } d_n =  \frac{\frac{2}{H} \int_0^H g_1(y) \sin \left( \frac{ n\pi y}{ H} \right) dy }{\sinh\left(\frac{-n\pi L}{H } \right) }
\end{align*}
\begin{note}[]
	At the corners we have $ u(0,0)=u(L,0)=u(0,H)=u(L,H)=0$.
\end{note}
\begin{intuition}
Recall the formal solution $ u(x,y)$ from above. We can show if  $ 0<a<b \implies \frac{\sinh(na)}{\sinh(nb) }< e^{n(a-b)}$ and $ e^{n(a-b)}<1$. Since $ x<L$ and  $ y<H$, the coefficients are finite integral of quotient of two hyperbolic terms (less than 1) and thus are bounded. We can show convergence along this line of logic.
\end{intuition}

\newpage
\section{Laplace in Circular Geometry}

We now wish to determine the formula for Laplace's equation in terms of the polar coordinates. Let's denote $ u(x,y)=v(r, \theta)$. Suppose $ x=r \cos(\theta ), y=r \sin(\theta )$. Then
\[
	\Delta u = \frac{1}{r} \frac{\partial }{\partial r} \left(r \frac{\partial v}{\partial r} \right) + \frac{1}{r^2} \frac{\partial^2 v}{\partial { \theta}^2}, r>0
.\] 
Using the Chain rule,
\[
\frac{\partial v}{\partial r} = \frac{\partial u}{\partial r} = \frac{\partial u}{\partial x} \cdot \frac{\partial x}{\partial r} + \frac{\partial u}{\partial y} \cdot \frac{\partial y}{\partial r} = u_x \cos(\theta ) + u_y \sin(\theta )
.\] 
and
\[
	\frac{\partial v}{\partial \theta} = \frac{\partial u}{\partial \theta} = u_x(-r \sin\theta) + u_y(r \cos\theta)  
.\] 
Now for the 2nd partials, we use the rules we discovered above:
\begin{align*}
	\frac{\partial^2 v}{\partial { r}^2} &= \frac{\partial }{\partial r} [u_x \cos\theta + u_y \sin\theta] \\
					     &= \frac{\partial }{\partial r} [u_x \cos\theta] + \frac{\partial }{\partial r} [u_y \sin\theta] \\
					     &= [u_{x x}\cos^2\theta + u_{xy} \cos \theta \sin\theta ]+ [u_{yx} \cos\theta \sin\theta + u_{yy}\sin^2\theta] \\
					     &= u_{x x} \cos^2\theta + 2u_{xy}\cos\theta \sin\theta + u_{yy} \sin^2\theta 
\end{align*}
Again doing this for $ \theta$,
\[
	\frac{\partial^2 v}{\partial { \theta}^2} = \frac{\partial }{\partial t} [u_x (-r \sin\theta)] + \frac{\partial }{\partial t} [u_y (r\cos\theta)]
.\] 
Thus by product rule, we eventually obtain
\[
	\frac{\partial^2 v}{\partial { \theta}^2} = u_{x x} r^2 \sin^2\theta - 2u_{yx}r^2 \cos\theta\sin\theta + u_{yy} r^2 \cos^2\theta - r(u_x \cos\theta+ u_y \sin\theta)
.\] 
dividing both sides by $ r^2$ yields:
\[	\frac{1}{r^2} \frac{\partial^2 v}{\partial { \theta}^2} = u_{x x} \sin^2\theta - 2u_{yx} \cos\theta\sin\theta + u_{yy} \cos^2\theta - \frac{1}{r} (u_x \cos\theta+ u_y \sin\theta)
.\]
Therefore, if we add these two second partials together:
\[
v_{rr} + \frac{1}{r^2} \cdot v_{\theta \theta} = u_{x x} + u_{yy} - \frac{1}{r}v_r
.\] 
This gives us
\[
\Delta u = u_{x x}+ u_{yy} = v_{rr} + \frac{1}{r}v_r + \frac{1}{r^2} v_{\theta \theta}
.\] 

\end{document}
